Began more fancy sparsity constructions

LogicalRefinement/Stlc/Interp.lean
@@ -52,11 +52,34 @@ def Context.sparsity: Context -> Sparsity
 | H::Hs => H.sparsity::(sparsity Hs)
 
 @[simp]
+def Sparsity.dep: Sparsity -> Nat -> Bool
+| [], n => true
+| b::Hs, 0 => b
+| b::Hs, Nat.succ n => dep Hs n
+
+theorem Sparsity.dep_get? {Γ: Sparsity} {n b}
+  : Γ.get? n = some b -> Γ.dep n = b
+  := by {
+    revert n;
+    induction Γ with
+    | nil => intro n H; cases H
+    | cons H Γ I =>
+      intro n Hn;
+      cases n with
+      | zero => simp [List.get?] at Hn; simp [Hn]
+      | succ n => simp only [dep, I Hn]
+  }
+
+def Sparsity.wknth: Sparsity -> Nat -> Bool -> Sparsity
+| H::Γ, Nat.succ n, b => H::(wknth Γ n b)
+| [], Nat.succ n, b => true::(wknth [] n b)
+| Γ, 0, b => b::Γ
+
+@[simp]
 def Sparsity.ix: Sparsity -> Nat -> Nat
-| _, 0 => 0
-| [], n => n
 | true::Hs, Nat.succ n => (ix Hs n) + 1
 | false::Hs, Nat.succ n => ix Hs n
+| _, n => n
 
 @[simp]
 def Sparsity.ix_inv: Sparsity -> Nat -> Nat
@@ -65,11 +88,11 @@ def Sparsity.ix_inv: Sparsity -> Nat -> Nat
 | _, n => n
 
 def Sparsity.ix_inv_valid (Γ: Sparsity) {n: Nat}:
-  Γ.get? n = some true -> Γ.ix_inv (Γ.ix n) = n
+  Γ.dep n = true -> Γ.ix_inv (Γ.ix n) = n
   := by {
     revert n;
     induction Γ with
-    | nil => intro n H; contradiction
+    | nil => intro n H; rfl
     | cons H Γ I =>
       intro n;
       cases n with
@@ -87,7 +110,7 @@ def Context.stlc_ix (Γ: Context): Nat -> Nat := Γ.sparsity.ix
 
 def Term.stlc: Term -> Sparsity -> Stlc
 | var n, σ => 
-  if σ.get? n = some true 
+  if σ.dep n
   then Stlc.var (σ.ix n) 
   else Stlc.abort
 | const TermKind.nil, _ => Stlc.nil
@@ -195,7 +218,7 @@ theorem HasVar.stlc {Γ A n}:
             | gst => exact (I Hv)
   }
 
-theorem HasVar.sigma {Γ A n s}:
+theorem HasVar.sigma_get? {Γ A n s}:
   HasVar Γ n (HypKind.val s) A ->
   Γ.sparsity.get? n = some (s == type)
   := by {
@@ -214,6 +237,15 @@ theorem HasVar.sigma {Γ A n s}:
       cases Γ <;> cases Hv
       rw [<-I (by assumption)]
       rfl
+  }
+
+theorem HasVar.sigma {Γ A n s}:
+  HasVar Γ n (HypKind.val s) A ->
+  Γ.sparsity.dep n = (s == type)
+  := by {
+    intro H;
+    apply Sparsity.dep_get?;
+    exact H.sigma_get?
   }
 
 -- But why...
@@ -278,4 +310,13 @@ theorem HasType.stlc {Γ a A}:
         cases Habs <;> assumption
         )
       )
+  }
+
+  theorem Term.stlc_wknth_false {t: Term} {Γ: Sparsity} {n: Nat}
+  : (t.wknth n).stlc (Γ.wknth n false) = t.stlc Γ
+  := by {
+    revert Γ n;
+    induction t with
+    | var v => sorry
+    | _ => sorry
   }
